(1) Find the explicit formula for $a_n$, where
    $a_n = 2^n - 4a_{n-1} - 4a_{n-2}$, with
    $a_0 = 1$ and $a_1 = 2$.\\

    \textit{(Solution)}\\

    If $a(n)$ be considered a generating function
    whose solution represents the $n^{th}$ value ($a_n$),
    this recursion can be expressed as a
    non-homogeneous advancement operator
    equation on $a$ as $(A^2+4A+4)a = 2^n$
    with $a(0)=1$ and $a(1)=2$. Or
    \begin{equation}
        (A+2)^2a=2^n
    \end{equation}
    
    Let's first consider the homogeneous part:
    \begin{equation}
        (A+2)^2a=0
    \end{equation}
    
    Since (2) is a polynomial of degree
    2, it must have a solution of the form of 2-parameters.
    One particular solution appears from the equality
    $(A+2)a=0$ or $Aa = -2a$. This is an advancement operator
    that multiplies the value of the function by $-2$
    at each succession. Hence the particular solution
    is $a_1=(-2)^n$. Let's try the other particular solution to be
    $a_2=n(-2)^n$:
    \begin{align*}
        (A+2)^2a_2 &= (A+2)(A+2)a_2\\
        &= (A+2)(A+2)n(-2)^n\\
        &= (A+2)\left[
            (n+1)(-2)^{n+1} + 2n(-2)^n
            \right]\\
        &= (n+2)(-2)^{n+2} + 2(n+1)(-2)^{n+1}
        + 2(n+1)(-2)^{n+1} + 4n(-2)^n\\
        &= (n+2)(-2)^{n+2} 
        + 4(n+1)(-2)^{n+1}
        + 4n(-2)^n\\
        &= (n+2)(-2)^{n+2} 
        - 2(n+1)(-2)^{n+2}
        + 4n(-2)^n\\
        &= -n(-2)^{n+2} 
        + 4n(-2)^n\\
        &= -4n(-2)^{n} 
        + 4n(-2)^n\\
        &= 0
    \end{align*}
    Hence the homogeneous part of the solution to (1),
    $a_h=c_1(-2)^n + c_2n(-2)^n$. Now for the non-homogeneous
    part, let's try a few particular solutions:\\

    \textit{guess \#1}:
    \begin{align*}
        a_{nh} &= c_32^n
        \text{. Plugging it into (1):}\\
        c_32^n &= 2^n - 4c_32^{n-1} - 4c_32^{n-2}\\
        &= 2^n - 2c_32^{n} - c_32^{n}\\
        &= 2^n - 3c_32^{n}\\
        c_3 & = \frac{1}{4}\\
    \end{align*}
    The explicit formula for $a_n$ is given by combining
    the homogeneous and the non-homogeneous parts:
    \begin{align*}
        a_n &= c_1(-2)^n + c_2n(-2)^n+\frac{2^n}{4}\\
        1 &= c_1 + 0 + \frac{1}{4},
        2 = c_1(-2) + c_2(1)(-2) + \frac{2}{4}
        \text{, using initial conditions.}\\
        c_1 &= \frac{3}{4}, c_2=-\frac{3}{2}\\
        a_n &= (-2)^n(\frac{3}{4} - \frac{3n}{2}) + \frac{2^n}{4}\\
        &= \boxed{(-2)^n(\frac{6-3n}{4}) + \frac{2^n}{4}}
    \end{align*}
    