\documentclass{article}
\usepackage{amsmath,amssymb}
\usepackage{mathtools}
\usepackage{amsfonts}
\usepackage{amssymb}
\usepackage{tikz}
\usepackage{enumitem}

\DeclarePairedDelimiter{\ceil}{\lceil}{\rceil}
\newcounter{question}
\setcounter{question}{0}
\begin{document}

\newcommand\Que[1]{%
   \leavevmode\par
   \stepcounter{question}
   \noindent
   \thequestion. Q --- #1\par}

\newcommand\Ans[2][]{%
    \leavevmode\par\noindent
   {\leftskip37pt
    A --- \textbf{#1}#2\par}}

\Que{
    For each generating function below, give a closed
    form for the $n^{th}$ term of its associated sequence.
    }
\Ans{
    Selected answers:
    \begin{enumerate}[label=\alph*]
        \item[a)]{
            \begin{align*}
                (1+x)^{10}
                & = \Sigma_{n=0}^{\infty} {10 \choose n} x^n
                && \text{(Newton's Binomial Theorem)}
            \end{align*}
            Therefore coefficient of the $n^{th}$ term:\\

            $\boxed{a_n = {10 \choose n} }$\\
        }
        \item[b)]{
            \begin{align*}
                \frac{1}{1-x^4}
                & = \frac{1}{(1-x)(1+x)(1+x^2)}\\
                & = \frac{A}{(1-x)} + \frac{B}{(1+x)} + \frac{Cx+D}{(1+x^2)}\\
                & = \frac{A(1+x)(1+x^2) + B(1-x)(1+x^2) + (Cx+D)(1-x^2)}{1-x^4}
                && \text{(for all $x$)}\\
                & \text{for $x=1$}, 4A = 1 \therefore \boxed{A=\frac{1}{4}}\\
                & \text{for $x=-1$}, 4B = 1 \therefore \boxed{B=\frac{1}{4}}\\
                & \text{ substituting:}\\
                & (1+x)(1+x^2) + (1-x)(1+x^2)+4(Cx+D)(1-x^2) = 4\\
                & x^3(-4C) + x^2(2-4D) + x(4C) + 4D = 2\\
                & \therefore \boxed{C=0}, \boxed{D=\frac{1}{2}}\\
                \frac{1}{1-x^4}
                & = \frac{1}{4(1-x)} + \frac{1}{4(1+x)} + \frac{1}{2(1+x^2)}\\
            \end{align*}
            We know that
            \begin{equation}
                \frac{1}{1-x} = 1+x+x^2+x^3+\dots
            \end{equation}

            Substituting $-x$ for $x$,
            \begin{equation}
                \frac{1}{1+x} = 1-x+x^2-x^3+\dots
            \end{equation}

            Differentiating (2) w.r.t $x$,
            \begin{align*}
                \frac{d}{dx} (\frac{1}{1+x})
                & = \frac{-1}{(1+x)^2}\\
                & = -1+2x-3x^2+\dots
            \end{align*}
            \begin{equation}
                \therefore \frac{1}{(1+x)^2} 
                = 1-2x+3x^2-\dots\\
            \end{equation}

            \begin{align*}
                \frac{1}{1-x^4}
                & = \frac{1}{4} (1+x+x^2+x^3+\dots)
                + \frac{1}{4} (1-x+x^2-x^3+\dots)
                + \frac{1}{2} (1-2x+3x^2-\dots)\\
                & = \frac{1}{4} (2+2x^2+2x^4+\dots)
                + \frac{1}{2} (1-2x+3x^2-\dots)\\
                & = \frac{1}{2} (1+x^2+x^4+\dots)
                + \frac{1}{2} (1-2x+3x^2-\dots)\\
                & = \frac{1}{2} (2-2x+4x^2-4x^3+6x^4-\dots)\\
                & = 1-x+2x^2-2x^3+3x^4-\dots\\
                & = \Sigma_{n=0}^{\infty}
                    (-1)^n (n+\frac{1+(-1)^n}{2})) x^n\\
                & = \Sigma_{n=0}^{\infty}
                    (-1)^n \frac{2n+1+(-1)^n}{2} x^n
            \end{align*}
            Therefore coefficient of the $n^{th}$ term:\\

            $\boxed{a_n = (-1)^n \frac{2n+1+(-1)^n}{2} }$\\
            }
        \item[e)]{
            \begin{align*}
                \frac{1+x^2-x^4}{1-x}\\
                & = \frac{1}{1-x} + \frac{x^2}{1-x} - \frac{x^4}{1-x}\\
                & = (1+x+x^2+x^3+\dots)
                + x^2(1+x+x^2+x^3+\dots)
                - x^4(1+x+x^2+x^3+\dots)\\
                & = \Sigma^{\infty} x^n
                + \Sigma^{\infty} x^{n+2}
                - \Sigma^{\infty} x^{n+4}
            \end{align*}
            Therefore coefficient of the $n^{th}$ term:\\

            $\boxed{a_n =  ?}$\\
        }
    \end{enumerate}
    }
\end{document}