\documentclass{article}
\usepackage{amsmath,amssymb}
\usepackage{mathtools}
\usepackage{amsfonts}
\usepackage{amssymb}
\usepackage{tikz}

\DeclarePairedDelimiter{\ceil}{\lceil}{\rceil}
\newcounter{question}
\setcounter{question}{0}
\begin{document}

\newcommand\Que[1]{%
   \leavevmode\par
   \stepcounter{question}
   \noindent
   \thequestion. Q --- #1\par}

\newcommand\Ans[2][]{%
    \leavevmode\par\noindent
   {\leftskip37pt
    A --- \textbf{#1}#2\par}}

\Que{
    Find an explicit formula for the recurrence:\\

    $a_0=5, a_{n+1}=2a_{n}-2, n\ge1$
    }
\Ans{
    The recurrence can be re-written as a 
    \textbf{nonhomogenous advancement operator equation}:\\

    $p(A)a = (A-2)a = -2$\\

    $p(A)$ only has one root, $A=2$. 
    A general solution to a homogenous equation of this
    form is:\\

    $a_1(n) = c{2}^n$\\

    Let's try $a_0(n) = d(-2)^n$ from the R.H.S of the original equation.\\

    \begin{align*}
        (A-2)a_0(n) & = (A-2)d(-2)^n\\
        & = d(-2)^{n+1} - 2d(-2)^n\\
        & = d(-2)^{n+1} + d(-2)^{n+1}\\
        & = 2d(-2)^{n+1}.\\
    \end{align*}

    If this were a solution to the nonhomogenous
    equation,\\
    
    $(A-2)a_0(n) = 2d(-2)^{n+1} = -2$\\
    
    $\therefore d = -(-2)^{-n-1}$\\

    Hence the general solution to the equation is:\\

    $a(n) = a_1(n)+a_0(n) = -(-2)^{-n-1} + c2^n$\\

    Since $a(0) = 5 = -(-2)^{-1} + c$,\\

    $c = 5 + (-2)^{-1} = 5 - 1/2 = 9/2$\\

    Therefore the exact formula for $a(n)$ is:\\

    \begin{align*}
        a(n) & = \frac{9}{2}2^{n} - (-2)^{-n-1}\\
        & = \frac{9}{2^{n+1}}2^{2n} - \frac{(-1)^{n+1}}{2^{n+1}}\\
        & = \boxed{\frac{9.2^{2n} + (-1)^n}{2^{n+1}}}\\
    \end{align*}
    }
\end{document}